[typing] refactorings

template-coq/theories/AstUtils.v
@@ -159,6 +159,45 @@ Proof.
   intro Heq; specialize (H0 Heq). discriminate.
 Qed.
 
+Definition eq_string s s' :=
+  if string_compare s s' is Eq then true else false.
+
+Definition eq_ind i i' :=
+  let 'mkInd i n := i in
+  let 'mkInd i' n' := i' in
+  eq_string i i' && Nat.eqb n n'.
+
+Definition eq_constant := eq_string.
+
+Definition eq_nat := Nat.eqb.
+Definition eq_evar := eq_nat.
+Definition eq_projection p p' :=
+  let '(ind, pars, arg) := p in
+  let '(ind', pars', arg') := p' in
+  eq_ind ind ind' && eq_nat pars pars' && eq_nat arg arg'.
+
+Lemma eq_string_refl x : eq_string x x = true.
+Proof.
+  unfold eq_string.
+  now rewrite (proj2 (string_compare_eq x x) eq_refl).
+Qed.
+
+Lemma eq_ind_refl i : eq_ind i i = true.
+Proof.
+  destruct i as [mind k].
+  unfold eq_ind. now rewrite eq_string_refl Nat.eqb_refl.
+Qed.
+
+Lemma eq_nat_refl n : eq_nat n n = true.
+Proof. by rewrite /eq_nat Nat.eqb_refl. Qed.
+
+Lemma eq_projection_refl i : eq_projection i i = true.
+Proof.
+  destruct i as [[mind k] p].
+  unfold eq_projection.
+  now rewrite eq_ind_refl !eq_nat_refl.
+Qed.
+
 Definition decompose_app (t : term) :=
   match t with
   | tApp f l => (f, l)
